Correctness.thy
@@ -1,325 +1,73 @@
 theory Correctness
-  imports "Denotational-Props" Launchbury
+  imports "CorrectnessStacked" "Launchbury-Unstack"
 begin
-
-lemma preserve_meaning:
-  assumes "\<Gamma> : e \<Down>\<^bsub>L\<^esub> \<Delta> : z"
-  and "x \<in> set L"
-  and "\<lbrace>\<Gamma>\<rbrace>\<rho> \<le> \<lbrace>\<Delta>\<rbrace>\<rho>"
-  shows "\<lbrakk>Var x\<rbrakk>\<^bsub>\<lbrace>\<Gamma>\<rbrace>\<rho>\<^esub> = \<lbrakk>Var x\<rbrakk>\<^bsub>\<lbrace>\<Delta>\<rbrace>\<rho>\<^esub>"
-proof(cases "x \<in> heapVars \<Gamma>")
-case True
-  thus ?thesis
-  using fmap_less_eqD[OF `\<lbrace>\<Gamma>\<rbrace>\<rho> \<le> \<lbrace>\<Delta>\<rbrace>\<rho>`, of x] 
-  by (auto simp add: heapVars_def)
-next
-case False with reds_avoids_live[OF assms(1,2)]
-  have "\<lbrakk>Var x\<rbrakk>\<^bsub>\<lbrace>\<Gamma>\<rbrace>\<rho>\<^esub> = the (lookup \<rho> x)" and "\<lbrakk>Var x\<rbrakk>\<^bsub>\<lbrace>\<Delta>\<rbrace>\<rho>\<^esub> = the (lookup \<rho> x)"
-    by (auto intro:  the_lookup_HSem_other simp add: heapVars_def)
-  thus ?thesis by simp
-qed
-
-inductive refines where
-  refinesI: "heapExtendJoin_cond' \<Gamma> ESem \<rho> \<Longrightarrow> (\<And> x e. (x, e) \<in> set \<Gamma> \<Longrightarrow> x \<in> fdom \<rho> \<Longrightarrow> the (lookup \<rho> x) \<sqsubseteq> \<lbrakk>e\<rbrakk>\<^bsub>\<lbrace>\<Gamma>\<rbrace>\<rho>\<^esub>)
-      \<Longrightarrow> refines \<Gamma> \<rho>"
-
-lemma refinesD:
-  assumes "refines \<Gamma> \<rho>"
-  assumes "(x, e) \<in> set \<Gamma>"
-  assumes "x \<in> fdom \<rho>"
-  shows "the (lookup \<rho> x) \<sqsubseteq> \<lbrakk>e\<rbrakk>\<^bsub>\<lbrace>\<Gamma>\<rbrace>\<rho>\<^esub>"
-using assms
- by (metis refines.simps)
-
-lemma refinesD':
-  assumes "refines \<Gamma> \<rho>"
-  assumes "finite S"
-  assumes "(x, e) \<in> set \<Gamma>"
-  assumes "x \<in> fdom \<rho> \<union> S"
-  shows "the (lookup (fmap_expand \<rho> (fdom \<rho> \<union> S)) x) \<sqsubseteq> \<lbrakk>e\<rbrakk>\<^bsub>\<lbrace>\<Gamma>\<rbrace>\<rho>\<^esub>"
-  using assms
-  apply (cases "x \<in> fdom \<rho>")
-  apply (auto dest: refinesD)
-  done
-
-lemma refines_is_heapExtendJoin_cond:
-  assumes "refines \<Gamma> \<rho>"
-  shows "heapExtendJoin_cond' \<Gamma> ESem \<rho>" (is "fix_on_cond_jfc' ?\<rho> ?F")
-  using assms
- by (metis refines.simps)
-(*
-proof (rule fix_on_cond_jfc'I[OF cont_compose[OF fmap_expand_cont cont2cont_heapToEnv[OF ESem_cont]]])
-  fix i
-  have compat: "compatible ?\<rho> (?F ?\<rho>)"
-    apply (rule compatible_fmap_expand)
-    apply simp
-    apply (rule ub_implies_compatible[OF _ below_refl])
-    apply (erule lookupHeapToEnvE)
-    apply (rule below_trans)
-    apply (erule (1) refinesD[OF assms,rotated, of _  _"fst ` set \<Gamma>"])
-    apply simp+
-    done
-  show "compatible ?\<rho> (?F (((\<lambda> \<rho>'. ?\<rho> \<squnion> ?F \<rho>')^^i) (to_bot ?\<rho>)))"
-  proof(induct i)
-  case 0 show ?case
-    apply simp
-    apply (rule ub_implies_compatible[of _ "?\<rho> \<squnion> ?F ?\<rho>"])
-    apply (rule join_above1[OF compat])
-    apply (rule below_trans[OF _ join_above2[OF compat]])
-    apply (rule cont2monofunE[OF cont_compose[OF fmap_expand_cont cont2cont_heapToEnv[OF ESem_cont]] to_bot_minimal])
-    done
-  case (Suc i)
-    show ?case
-    apply (rule compatible_fmap_expand)
-    apply simp
-    apply (rule ub_implies_compatible[OF _ below_refl])
-    apply (erule lookupHeapToEnvE)
-    apply (rule below_trans)
-    apply (erule (1) refinesD[OF assms,rotated, of _  _"fst ` set \<Gamma>"])
-    apply simp
-    apply simp
-    apply (rule cont2monofunE[OF ESem_cont join_above1[OF Suc]])
-    done
-  qed
-qed
-*)
-
-(*
-lemma refines_subsetD:
-  "refines \<Gamma> \<rho> \<Longrightarrow> set \<Delta> \<subseteq> set \<Gamma> \<Longrightarrow> refines \<Delta> \<rho>"
-  apply (rule refinesI)
-  apply (drule refines_is_heapExtendJoin_cond)
-  apply (frule (1) subsetD)
-  apply (drule (3) refinesD)
-  apply assumption
-  done
-*)
-
-
-lemma refines_insertI:
-  assumes "refines \<Gamma> \<rho>"
-  assumes "heapExtendJoin_cond' ((x, e) # \<Gamma>) ESem \<rho>"
-  assumes "x \<in> fdom \<rho> \<Longrightarrow> the (lookup \<rho> x) \<sqsubseteq> \<lbrakk>e\<rbrakk>\<^bsub>\<lbrace>(x,e) # \<Gamma>\<rbrace>\<rho>\<^esub>"
-  shows "refines ((x,e) # \<Gamma>) \<rho>"
-proof(rule refinesI[OF assms(2)])
-  case (goal1 x' e')
-  show ?case
-  proof(cases "(x', e') = (x, e)")
-  case True
-    with goal1 have "x \<in> fdom \<rho>" by auto
-    from assms(3)[OF this]
-    show ?thesis using True by simp
-  next
-  case False
-    hence "(x', e') \<in> set \<Gamma>" using goal1(1) by auto
-    from refinesD[OF assms(1) this goal1(2)]
-    show ?thesis
-      apply (rule below_trans)
-      apply (rule cont2monofunE[OF ESem_cont])
-      sorry
-(*    apply (rule HSem_mono_subset)
-      apply auto
-      done *)
-  qed
-qed
-
-lemma compatible_fmap_expand:
-  assumes "\<And> x. x \<in> fdom \<rho>1 \<Longrightarrow> x \<in> fdom \<rho>2 \<Longrightarrow> compatible (the (lookup \<rho>1 x)) (the (lookup \<rho>2 x))"
-  shows "compatible (fmap_expand \<rho>1 S) (fmap_expand \<rho>2 S)"
-  apply (case_tac "finite S")
-  apply (rule compatible_fmap_is_compatible[OF compatible_fmapI])
-  apply (case_tac "x \<in> fdom \<rho>1")
-  apply (case_tac "x \<in> fdom \<rho>2")
-  apply (auto simp add: assms fmap_expand_nonfinite)
-  done
 
 
 theorem correctness:
-  assumes "\<Gamma> : e \<Down>\<^bsub>L\<^esub> \<Delta> : z"
-  and "refines \<Gamma> \<rho>"
-  and "distinctVars \<Gamma>"
-  and "fdom \<rho> \<subseteq> set L"
-  shows "\<lbrakk>e\<rbrakk>\<^bsub>\<lbrace>\<Gamma>\<rbrace>\<rho>\<^esub> = \<lbrakk>z\<rbrakk>\<^bsub>\<lbrace>\<Delta>\<rbrace>\<rho>\<^esub>" and "\<lbrace>\<Gamma>\<rbrace>\<rho> \<le> \<lbrace>\<Delta>\<rbrace>\<rho>" and "refines \<Delta> \<rho>"
-  using assms
-proof(nominal_induct avoiding: \<rho>  rule:reds.strong_induct)
-print_cases
-case (Lambda \<Gamma> x e L \<rho>)
-  print_cases
-  case 1 show ?case by simp
-  case 2 show ?case by simp
-  case 3 show ?case by fact
-next
+  assumes "\<Gamma> : e \<Down>\<^bsub>x#L\<^esub> \<Delta> : z"
+  and [simp]:"distinctVars \<Gamma>"
+  and fresh: "atom x \<sharp> (\<Gamma>,e)"
+  shows "\<lbrakk>e\<rbrakk>\<^bsub>\<lbrace>\<Gamma>\<rbrace>fempty\<^esub> = \<lbrakk>z\<rbrakk>\<^bsub>\<lbrace>\<Delta>\<rbrace>fempty\<^esub>" and "\<lbrace>\<Gamma>\<rbrace>fempty \<le> \<lbrace>\<Delta>\<rbrace>fempty"
+proof-
 
-case (Application y \<Gamma> e x L \<Delta> \<Theta> z e' \<rho>)
+  have "\<Gamma> : [(x, e)] \<Down> \<Delta> : [(x, z)]"
+    by (rule add_stack[OF assms(1)], simp_all add: supp_Nil)
+  moreover
+  from `atom x \<sharp> (\<Gamma>,e)`
+  have "x \<notin> heapVars \<Gamma>"
+    by (metis heapVars_not_fresh fresh_Pair)
+  hence "distinctVars ([(x, e)] @ \<Gamma>)"
+    by (simp add: distinctVars_append distinctVars_Cons)
+  ultimately
+  have le: "\<lbrace>[(x, e)] @ \<Gamma>\<rbrace>fempty \<le> \<lbrace>[(x, z)] @ \<Delta>\<rbrace>fempty"
+    by (rule CorrectnessStacked.correctness)
+ 
+  have "atom x \<sharp> (\<Delta>, z)"
+    using reds_fresh[OF assms(1) fresh]
+    by auto
 
-  case 1
-  have "fdom \<rho> \<subseteq> set (x # L)" by (metis `fdom \<rho> \<subseteq> set L` set_subset_Cons subset_trans)
-  note Application.hyps(10,11,12)[OF `refines \<Gamma> \<rho>`  `distinctVars \<Gamma>` `fdom \<rho> \<subseteq> set (x # L)`]
-  note reds_pres_distinctVars[OF Application.hyps(9) `distinctVars \<Gamma>`]
-  note Application.hyps(14,15,16)[OF `refines \<Delta> \<rho>` `distinctVars \<Delta>` `fdom \<rho> \<subseteq> set L`]
-  have "\<lbrakk> App e x \<rbrakk>\<^bsub>\<lbrace>\<Gamma>\<rbrace>\<rho>\<^esub> = \<lbrakk> e \<rbrakk>\<^bsub>\<lbrace>\<Gamma>\<rbrace>\<rho>\<^esub> \<down>Fn \<lbrakk> Var x \<rbrakk>\<^bsub>\<lbrace>\<Gamma>\<rbrace>\<rho>\<^esub>"
-    by simp also
-  have "... = \<lbrakk> Lam [y]. e' \<rbrakk>\<^bsub>\<lbrace>\<Delta>\<rbrace>\<rho>\<^esub> \<down>Fn \<lbrakk> Var x \<rbrakk>\<^bsub>\<lbrace>\<Gamma>\<rbrace>\<rho>\<^esub>"
-    using `\<lbrakk> e \<rbrakk>\<^bsub>\<lbrace>\<Gamma>\<rbrace>\<rho>\<^esub> = _` by simp also
-  have "... = \<lbrakk> Lam [y]. e' \<rbrakk>\<^bsub>\<lbrace>\<Delta>\<rbrace>\<rho>\<^esub> \<down>Fn \<lbrakk> Var x \<rbrakk>\<^bsub>\<lbrace>\<Delta>\<rbrace>\<rho>\<^esub>"
-    by (subst preserve_meaning[OF `\<Gamma> : e \<Down>\<^bsub>x # L\<^esub> \<Delta> : Lam [y]. e'` _ `\<lbrace>\<Gamma>\<rbrace>\<rho> \<le> \<lbrace>\<Delta>\<rbrace>\<rho>`], auto) also
-  have "... = (\<Lambda> v. \<lbrakk> e' \<rbrakk>\<^bsub>(\<lbrace>\<Delta>\<rbrace>\<rho>)(y f\<mapsto> v)\<^esub>)\<cdot>(\<lbrakk> Var x \<rbrakk>\<^bsub>\<lbrace>\<Delta>\<rbrace>\<rho>\<^esub>)"
-    using `atom y \<sharp> \<Delta>` and `atom y \<sharp> \<rho>` by simp also
-  have "... = \<lbrakk> e' \<rbrakk>\<^bsub>(\<lbrace>\<Delta>\<rbrace>\<rho>)(y f\<mapsto> (\<lbrakk> Var x \<rbrakk>\<^bsub>\<lbrace>\<Delta>\<rbrace>\<rho>\<^esub>))\<^esub>"
-    by simp also
-  have "... = \<lbrakk>  e'[y::=x] \<rbrakk>\<^bsub>(\<lbrace>\<Delta>\<rbrace>\<rho>)\<^esub>"
-    using `atom y \<sharp> \<Delta>` and `atom y \<sharp> \<rho>` and `atom y \<sharp> x`
-    by-(rule ESem_subst, simp_all add:fresh_at_base) also
-  have "... = \<lbrakk> z \<rbrakk>\<^bsub>\<lbrace>\<Theta>\<rbrace>\<rho>\<^esub>"
-    using `\<lbrakk>  e'[y::=x] \<rbrakk>\<^bsub>_\<^esub> = _` by simp
-  finally
-  show ?case .
-  case 2 show ?case using `\<lbrace>\<Gamma>\<rbrace>\<rho> \<le> _` `\<lbrace>\<Delta>\<rbrace>\<rho> \<le> _`  by simp
-  case 3 show ?case by fact
-next
+  have "\<lbrace>\<Gamma>\<rbrace>fempty = fmap_restr (fst ` set \<Gamma>) (\<lbrace>(x, e) # \<Gamma>\<rbrace>fempty)"
+    apply (rule HSem_add_fresh[of fempty, simplified (no_asm), unfolded heapVars_def, symmetric])
+    apply (rule fempty_is_heapExtendJoin_cond'_ESem)
+    apply (rule fempty_is_heapExtendJoin_cond'_ESem)
+    using fresh apply (simp add: fresh_Pair)
+    done
+  also have "... \<le> fmap_restr (fst ` set \<Delta>) (\<lbrace>(x, z) # \<Delta>\<rbrace>fempty)"
+    by (rule fmap_restr_le[OF le reds_doesnt_forget[unfolded heapVars_def, OF assms(1)], simplified])
+  also have "... = \<lbrace>\<Delta>\<rbrace>fempty"
+    apply (rule HSem_add_fresh[of fempty, simplified (no_asm), unfolded heapVars_def])
+    apply (rule fempty_is_heapExtendJoin_cond'_ESem)
+    apply (rule fempty_is_heapExtendJoin_cond'_ESem)
+    using `_ \<sharp> (\<Delta>,z)` apply (simp add: fresh_Pair)
+    done
+  finally show "\<lbrace>\<Gamma>\<rbrace>fempty \<le> \<lbrace>\<Delta>\<rbrace>fempty".
+ 
 
-case (Variable x e \<Gamma> L \<Delta> z \<rho>)
-  have xnot1: "x \<notin> fst ` set (removeAll (x, e) \<Gamma>)" sorry
-  hence xnot2: "x \<notin> fst ` set \<Delta>"
-    by (rule reds_avoids_live[OF `removeAll (x, e) \<Gamma> : e \<Down>\<^bsub>x#L\<^esub> \<Delta> : z`, unfolded heapVars_def, rotated], simp)
-
-  assume "refines \<Gamma> \<rho>"
-  hence "refines (removeAll (x, e) \<Gamma>) \<rho>" sorry (* by (auto intro: refines_subsetD) *)
-  assume "fdom \<rho> \<subseteq> set L" 
-  hence "fdom \<rho> \<subseteq> set (x # L)" by (metis set_subset_Cons subset_trans)
-
-  assume "distinctVars \<Gamma>"
-  hence "distinctVars (removeAll (x, e) \<Gamma>)"
-    by (rule distinctVars_removeAll[OF _  `(x, e) \<in> set \<Gamma>`])
-
-  note hyps = Variable.hyps(3-5)[OF `refines (removeAll (x, e) \<Gamma>) \<rho>` `distinctVars (removeAll (x, e) \<Gamma>)` `fdom \<rho> \<subseteq> set (x#L)`]
-
-  thm refinesD[OF `refines \<Gamma> \<rho>` `(x,e) \<in> set \<Gamma>`]
-
-  from `refines \<Delta> \<rho>`
-  have "refines ((x, z) # \<Delta>) \<rho>"
-    (*
-    apply (rule refines_insertI)
-    apply (rule below_trans)
-    apply (erule (1) refinesD[OF `refines \<Gamma> \<rho>` _ `(x,e) \<in> set \<Gamma>`])
-    find_theorems e z
-    *)
-  sorry
-
-  have cond: "heapExtendJoin_cond' \<Gamma> ESem \<rho>"
-    by (rule refines_is_heapExtendJoin_cond, fact)
-
-  have cond: "heapExtendJoin_cond' ((x, e) # removeAll (x, e) \<Gamma>) ESem \<rho>"
-    (* simple consequence of set being equal *)
-    sorry
-  have cond2: "heapExtendJoin_cond' ((x, z) # \<Delta>) ESem \<rho>"
-    by (rule refines_is_heapExtendJoin_cond, fact)
-
-  let "?S" = "(fix_join_compat'' (fmap_expand \<rho> (fdom \<rho> \<union> fst ` set ((x, e) # removeAll (x, e) \<Gamma>)))
-       (\<lambda>\<rho>'a. fmap_expand (heapToEnv ((x, e) # removeAll (x, e) \<Gamma>) (\<lambda>e. \<lbrakk> e \<rbrakk>\<^bsub>\<rho>'a\<^esub>))
-               (fdom \<rho> \<union> fst ` set ((x, e) # removeAll (x, e) \<Gamma>))))"
-  let "?S2" = "(fix_join_compat'' (fmap_expand \<rho> (fdom \<rho> \<union> fst ` set ((x, z) # \<Delta>)))
-       (\<lambda>\<rho>'a. fmap_expand (heapToEnv ((x, z) # \<Delta>) (\<lambda>e. \<lbrakk> e \<rbrakk>\<^bsub>\<rho>'a\<^esub>))
-               (fdom \<rho> \<union> fst ` set ((x, z) # \<Delta>))))"
-
-  case 2
-  have "\<lbrace>\<Gamma>\<rbrace>\<rho> = \<lbrace>(x,e) # removeAll (x,e) \<Gamma>\<rbrace>\<rho>" sorry also (* Distinctness and reordering lemma needed *)
-  have "... = fix_on ?S
-     (\<lambda>\<rho>'. (\<lbrace>removeAll (x, e) \<Gamma>\<rbrace>\<rho>') \<squnion>
-            (fmap_bottom (fdom \<rho> \<union> fst ` set ((x, e) # removeAll (x, e) \<Gamma>))(x f\<mapsto> \<lbrakk> e \<rbrakk>\<^bsub>\<rho>'\<^esub>) \<squnion>
-             fmap_expand \<rho> (fdom \<rho> \<union> fst ` set ((x, e) # removeAll (x, e) \<Gamma>))))"                           
-    by (rule iterative_HSem[OF cond xnot1])
-  also
-  have "... = fix_on ?S
-     (\<lambda>\<rho>'. (\<lbrace>removeAll (x, e) \<Gamma>\<rbrace>\<rho>') \<squnion>
-            (fmap_bottom (fdom \<rho> \<union> fst ` set ((x, e) # removeAll (x, e) \<Gamma>))(x f\<mapsto> \<lbrakk> e \<rbrakk>\<^bsub>\<lbrace>removeAll (x, e) \<Gamma>\<rbrace>\<rho>'\<^esub>) \<squnion>
-             fmap_expand \<rho> (fdom \<rho> \<union> fst ` set ((x, e) # removeAll (x, e) \<Gamma>))))"                           
-    sorry also (* Unfolding a bit under the fixed point, as in 5.2.1 *)
-  have "... = fix_on ?S
-     (\<lambda>\<rho>'. (\<lbrace>removeAll (x, e) \<Gamma>\<rbrace>\<rho>') \<squnion>
-            (fmap_bottom (fdom \<rho> \<union> fst ` set ((x, e) # removeAll (x, e) \<Gamma>))(x f\<mapsto> \<lbrakk> z \<rbrakk>\<^bsub>\<lbrace>\<Delta>\<rbrace>\<rho>'\<^esub>) \<squnion>
-             fmap_expand \<rho> (fdom \<rho> \<union> fst ` set ((x, e) # removeAll (x, e) \<Gamma>))))"  
-   apply (rule fix_on_cong)
-   (* fix_on_cond with bit unfolded *)
-   defer
-   (* drule for refines in jfc'' *)
-   apply (rule arg_cong[OF Variable.hyps(3)])
-   defer
-   sorry also 
-   (*    by (subst  hyps(1), rule refl) also *)
-   have "... \<le> fix_on ?S
-     (\<lambda>\<rho>'. (\<lbrace>\<Delta>\<rbrace>\<rho>') \<squnion>
-            (fmap_bottom (fdom \<rho> \<union> fst ` set ((x, e) # removeAll (x, e) \<Gamma>))(x f\<mapsto> \<lbrakk> z \<rbrakk>\<^bsub>\<lbrace>\<Delta>\<rbrace>\<rho>'\<^esub>) \<squnion>
-             fmap_expand \<rho> (fdom \<rho> \<union> fst ` set ((x, e) # removeAll (x, e) \<Gamma>))))"
-    using Variable.hyps(4)
-    (* \<le> and fix1 *)
-    sorry also
-  have "... = fix_on ?S2
-     (\<lambda>\<rho>'. (\<lbrace>\<Delta>\<rbrace>\<rho>') \<squnion>
-            (fmap_bottom (fdom \<rho> \<union> fst ` set ((x, z) # \<Delta>))(x f\<mapsto> \<lbrakk> z \<rbrakk>\<^bsub>\<lbrace>\<Delta>\<rbrace>\<rho>'\<^esub>) \<squnion>
-             fmap_expand \<rho> (fdom \<rho> \<union> fst ` set ((x, z) # \<Delta>))))"
-    (* fdoms anpassen *)
-    sorry also
-  have "... = fix_on ?S2
-     (\<lambda>\<rho>'. (\<lbrace>\<Delta>\<rbrace>\<rho>') \<squnion>
-            (fmap_bottom (fdom \<rho> \<union> fst ` set ((x, z) # \<Delta>))(x f\<mapsto> \<lbrakk> z \<rbrakk>\<^bsub>\<rho>'\<^esub>) \<squnion>
-             fmap_expand \<rho> (fdom \<rho> \<union> fst ` set ((x, z) # \<Delta>))))"
-    (* Again 5.2.1 *)
-    sorry also
-  have  "... = \<lbrace>(x, z) # \<Delta>\<rbrace>\<rho>"
-    by (rule iterative_HSem[OF cond2  xnot2,symmetric])
-  finally show part2: ?case.
-
-  case 1
-  have "\<lbrakk> Var x \<rbrakk>\<^bsub>\<lbrace>\<Gamma>\<rbrace>\<rho>\<^esub> = the (lookup (\<lbrace>\<Gamma>\<rbrace>\<rho>) x)" by simp also
-  have "... = the (lookup (\<lbrace>(x, z) # \<Delta>\<rbrace>\<rho>) x)"
-    using part2 (* Definition of \<le> and existence of x in \<Gamma> *)
-    sorry also
-  have "... = \<lbrakk> z \<rbrakk>\<^bsub>\<lbrace>(x,z) # \<Delta>\<rbrace>\<rho>\<^esub>"
-    apply (subst HSem_unroll[OF cond2])
-    apply (subst the_lookup_join[OF rho_F_compat_jfc''[OF cond2 HSem_there[OF cond2]]])
-    apply auto
-    apply (rule larger_is_join)
-    apply (cases "x \<in> fdom \<rho>")
-    apply (rule refinesD'[OF `refines ((x, z) # \<Delta>) \<rho>`, of "fst ` set  ((x, z) # \<Delta>)", simplified])
-    apply auto[2]
+  have "\<lbrakk>e\<rbrakk>\<^bsub>\<lbrace>\<Gamma>\<rbrace>fempty\<^esub> = \<lbrakk>e\<rbrakk>\<^bsub>\<lbrace>(x, e) # \<Gamma>\<rbrace>fempty\<^esub>"
+    apply (rule ESem_add_fresh[symmetric])
+    apply (rule fempty_is_heapExtendJoin_cond'_ESem)
+    apply (rule fempty_is_heapExtendJoin_cond'_ESem)
+    using fresh by (simp add: fresh_Pair)
+  also have "... = the (lookup (\<lbrace>(x, e) # \<Gamma>\<rbrace>fempty) x)"
+    apply (rule the_lookup_HSem_heap[of _ "(x, e) # \<Gamma>" x, simplified (no_asm), symmetric])
+    apply (rule fempty_is_heapExtendJoin_cond'_ESem)
+    apply simp_all    
+    done
+  also have "... = the (lookup (\<lbrace>(x, z) # \<Delta>\<rbrace>fempty) x)"
+    apply (rule arg_cong[OF fmap_less_eqD[OF le, simplified]])
     apply simp
     done
-  finally show ?case.
-
-  case 3 show ?case by fact
-next
-
-case (Let as \<Gamma> L body \<Delta> z \<rho>)
-  assume "fdom \<rho> \<subseteq> set L"
-  note `set (bn as) \<sharp>* L`
-  hence "set (bn as) \<sharp>* set L"  by (metis fresh_star_set)
-  hence "set (bn as) \<sharp>* fdom \<rho>"
-    by (rule fresh_star_subset[OF finite_set _ `fdom \<rho> \<subseteq> set L`])
-  hence "set (bn as) \<sharp>* \<rho>"
-    by (simp add:fresh_def fresh_star_def supp_fmap pure_supp)
-  have "set (bn as) \<sharp>* (\<lbrace>\<Gamma>\<rbrace>\<rho>)"
-    by (rule fresh_star_fun_eqvt_app2[OF HSem_eqvt `set (bn as) \<sharp>* \<Gamma>` `set (bn as) \<sharp>* \<rho>`])
-
-  have "refines (asToHeap as @ \<Gamma>) \<rho>" sorry
- 
-  assume "distinctVars \<Gamma>"
-  note distinctVars_append_asToHeap[OF `distinctVars (asToHeap as)` `distinctVars \<Gamma>` `set (bn as) \<sharp>* \<Gamma>`]
-  note hyps = Let.hyps(5-7)[OF `refines (asToHeap as @ \<Gamma>) \<rho>` `distinctVars (asToHeap as @ \<Gamma>)` `fdom \<rho> \<subseteq> set L`]
-
-  case 1
-  have "\<lbrakk> Let as body \<rbrakk>\<^bsub>\<lbrace>\<Gamma>\<rbrace>\<rho>\<^esub> = \<lbrakk> body \<rbrakk>\<^bsub>\<lbrace>asToHeap as\<rbrace>\<lbrace>\<Gamma>\<rbrace>\<rho>\<^esub>"
-    by (rule Esem_simps4[OF `set (bn as) \<sharp>* (\<lbrace>\<Gamma>\<rbrace>\<rho>)`]) also
-  have "... = \<lbrakk> body \<rbrakk>\<^bsub>\<lbrace>asToHeap as @ \<Gamma>\<rbrace>\<rho>\<^esub>" sorry also
-  have "... = \<lbrakk> z \<rbrakk>\<^bsub>\<lbrace>\<Delta>\<rbrace>\<rho>\<^esub>" by (rule hyps)
-  finally show ?case .
-
-  case 2
-  have "\<lbrace>\<Gamma>\<rbrace>\<rho> \<le> \<lbrace>asToHeap as @ \<Gamma>\<rbrace>\<rho>" sorry also
-  have "... \<le> \<lbrace>\<Delta>\<rbrace>\<rho>" by (rule hyps)
-  finally show ?case .
-
-  case 3 show ?case by (rule hyps)
+  also have "... = \<lbrakk>z\<rbrakk>\<^bsub>\<lbrace>(x, z) # \<Delta>\<rbrace>fempty\<^esub>"
+    apply (rule the_lookup_HSem_heap[of _ "(x, z) # \<Delta>" x, simplified (no_asm)])
+    apply (rule fempty_is_heapExtendJoin_cond'_ESem)
+    apply simp_all    
+    done
+  also have "... =  \<lbrakk>z\<rbrakk>\<^bsub>\<lbrace>\<Delta>\<rbrace>fempty\<^esub>"
+    apply (rule ESem_add_fresh)
+    apply (rule fempty_is_heapExtendJoin_cond'_ESem)
+    apply (rule fempty_is_heapExtendJoin_cond'_ESem)
+    using `atom x \<sharp> (\<Delta>,z)` by (simp add: fresh_Pair)
+  finally show "\<lbrakk> e \<rbrakk>\<^bsub>\<lbrace>\<Gamma>\<rbrace>fempty\<^esub> = \<lbrakk> z \<rbrakk>\<^bsub>\<lbrace>\<Delta>\<rbrace>fempty\<^esub>".
 qed
 
 end
