Launchbury-Unstack.thy
@@ -2,6 +2,9 @@ theory "Launchbury-Unstack"
 imports Launchbury LaunchburyStacked
 begin
 
+lemma supp_set_mem: "x \<in> set L \<Longrightarrow> supp x \<subseteq> supp L"
+  by (induct L, auto simp add: supp_Cons)
+
 lemma forget_stack:
   assumes "\<Gamma> : \<Gamma>' \<Down> \<Delta> : \<Delta>'"
   and "supp S \<subseteq> supp (tl \<Gamma>')"
@@ -21,16 +24,28 @@ case (Application n \<Gamma> \<Gamma>' \<Delta> \<Delta>' x e y \<Theta> \<Theta
     using Application stack_not_empty[OF Application(24)]
     by (cases \<Theta>', auto simp add: fresh_Cons fresh_Pair)
   ultimately
-  have fresh: "atom z \<sharp> (\<Gamma>, e, y, S, \<Delta>, \<Theta>, snd (hd \<Theta>'))"
+  have fresh: "atom z \<sharp> (\<Gamma>, e, y, S, \<Delta>, \<Theta>, snd (hd \<Theta>'), n)"
     using Application
-    by (simp add: fresh_Pair fresh_Cons)[1]
+    by (simp add: fresh_Pair fresh_Cons fresh_at_base)[1]
 
-  have "supp (y # S) \<subseteq> supp ( (x, App (Var n) y) # \<Gamma>')"
+  have "atom n \<sharp> \<Gamma>'" using Application by (simp add: fresh_Pair)
+  hence "atom n \<sharp> map fst \<Gamma>'"
+    by (induct \<Gamma>')(auto simp add: fresh_Cons fresh_Nil)
+  moreover
+  have  "atom n \<sharp> snd (hd \<Theta>')"
+    using Application stack_not_empty[OF Application(24)]
+    by (cases \<Theta>', auto simp add: fresh_Cons fresh_Pair)
+  ultimately
+  have fresh2: "atom n \<sharp> (\<Gamma>, e, y, S, \<Delta>, \<Theta>, snd (hd \<Theta>'))"
+    using Application
+    by (simp add: fresh_Pair fresh_Cons fresh_at_base)[1]
+ 
+
+  have "supp (n # y # S) \<subseteq> supp ( (x, App (Var n) y) # \<Gamma>')"
     using Application.prems(1)
     by (auto simp add: supp_Cons supp_Pair exp_assn.supp)
-  hence hyp1: "\<Gamma> : e \<Down>\<^bsub>y # S\<^esub> \<Delta> : Lam [z]. e'" 
+  hence hyp1: "\<Gamma> : e \<Down>\<^bsub>n # y # S\<^esub> \<Delta> : Lam [z]. e'" 
     by (rule Application.hyps(23)[simplified])
-
   have "supp S \<subseteq> supp \<Delta>'"
     using Application.prems(1)
     using stack_unchanged[OF Application.hyps(22)]
@@ -39,7 +54,7 @@ case (Application n \<Gamma> \<Gamma>' \<Delta> \<Delta>' x e y \<Theta> \<Theta
     by (rule Application.hyps(25)[simplified])
    
   show ?case
-    by (simp, rule Launchbury.Application[OF fresh hyp1 hyp2])
+    by (simp, rule Launchbury.Application[OF fresh fresh2 hyp1 hyp2])
 next
 case (Variable y e \<Gamma> x \<Gamma>' \<Delta> z \<Delta>' S)
   have "supp (y # S) \<subseteq> supp ((x, Var y) # \<Gamma>')"
@@ -60,11 +75,79 @@ case (Let as \<Gamma> x body \<Gamma>' \<Delta> \<Delta>' S)
     using Let(4) using `supp S \<subseteq> supp \<Gamma>'`
     by (auto simp add: fresh_star_def fresh_def)
 
-  hence fresh: "set (bn as) \<sharp>* (\<Gamma>, S)"
+  hence fresh: "set (bn as) \<sharp>* (\<Gamma>, Terms.Let as body, S)"
     using Let by (auto simp add: fresh_star_Pair)
 
   show ?case
     by (simp, rule Launchbury.Let[OF fresh Let.hyps(5) hyp])
 qed
+
+lemma add_stack:
+  assumes "\<Gamma> : e \<Down>\<^bsub>L\<^esub> \<Delta> : z"
+  assumes "x \<in> set L"
+  assumes "supp \<Gamma>' \<subseteq> supp L"
+  shows "\<Gamma> : (x,e) # \<Gamma>' \<Down> \<Delta> : (x,z) # \<Gamma>'"
+using assms
+proof (nominal_induct avoiding: \<Gamma>' x rule: Launchbury.reds.strong_induct)
+case (Lambda \<Gamma> xa e L \<Gamma>')
+  show ?case
+    by (auto intro: reds.intros)
+next
+case (Application y \<Gamma> e xa L \<Delta> \<Theta> z n e' \<Gamma>' x)
+  have fresh_n: "atom n \<sharp> (\<Gamma>, \<Gamma>', \<Delta>, \<Gamma>', x, e, xa, \<Theta>, (x, z) # \<Gamma>', y)"
+    using Application
+    by (simp add: fresh_Pair fresh_Cons fresh_at_base)
+
+  have fresh_y: "atom y \<sharp> (\<Gamma>, \<Gamma>', \<Delta>, \<Gamma>', x, e, xa, \<Theta>, (x, z) # \<Gamma>')"
+    using Application
+    by (simp add: fresh_Pair fresh_Cons)
+
+  have "supp ((x, App (Var n) xa) # \<Gamma>') \<subseteq> supp (n # xa # L)"
+     using set_mp[OF supp_set_mem[OF `x \<in> set L`]] set_mp[OF `supp \<Gamma>' \<subseteq> supp L`]
+     by (auto simp add: supp_Pair supp_Cons exp_assn.supp)
+  hence hyp1: "\<Gamma> : (n, e) # (x, App (Var n) xa) # \<Gamma>' \<Down> \<Delta> : (n, Lam [y]. e') # (x, App (Var n) xa) # \<Gamma>'"
+    apply (rule Application(21)[rotated])
+    apply simp
+    done
+ 
+  have hyp2: "\<Delta> : (x, e'[y::=xa]) # \<Gamma>' \<Down> \<Theta> : (x, z) # \<Gamma>'"
+    apply (rule Application(23)[OF Application.prems])
+    done
+
+  show ?case
+    by (rule reds.Application[OF fresh_n fresh_y hyp1 hyp2])
+next
+case (Variable x e \<Gamma> L \<Delta> z \<Gamma>' xa)
+  have "supp ((xa, Var x) # \<Gamma>') \<subseteq> supp (x # L)"
+     using set_mp[OF supp_set_mem[OF `xa \<in> set L`]] set_mp[OF `supp \<Gamma>' \<subseteq> supp L`]
+     by (auto simp add: supp_Pair supp_Cons exp_assn.supp)
+  hence hyp: "removeAll (x, e) \<Gamma> : (x, e) # (xa, Var x) # \<Gamma>' \<Down> \<Delta> : (x, z) # (xa, Var x) # \<Gamma>'"
+    apply (rule Variable.hyps(3)[rotated])
+    apply (simp)
+    done
+  show ?case
+    by (rule reds.Variable[OF `(x,e) \<in> set _` hyp])
+next
+case (Let as \<Gamma> body L \<Delta> z \<Gamma>' x)
+  from `x \<in> set L` and `_ \<sharp>* L`
+  have [simp]:"set (bn as) \<sharp>* x"
+    by (metis fresh_star_Cons fresh_star_list(1) in_set_conv_decomp)
+
+  from `supp \<Gamma>' \<subseteq> supp L` and `_ \<sharp>* L`
+  have [simp]:"set (bn as) \<sharp>* \<Gamma>'"
+    by (auto simp add: fresh_star_def fresh_def)
+
+  have fresh: "set (bn as) \<sharp>* (\<Gamma>, x, Terms.Let as body, \<Gamma>')"
+    using Let(1-3)
+    by (simp add: fresh_star_Pair)
+ 
+  have hyp: "asToHeap as @ \<Gamma> : (x, body) # \<Gamma>' \<Down> \<Delta> : (x, z) # \<Gamma>'"
+    apply (rule Let.hyps(6)[OF Let.prems])
+    done
+
+  show ?case
+    by (rule reds.Let[OF fresh `distinctVars (asToHeap as)` hyp])
+qed
+
 
 end
